\begin{frame}


    \begin{columns}[T]
        \begin{column}{0.5\textwidth}
            \input{figures/xt_atildet}     
%            \vspace{-0.5cm}
            \begin{align*}
                \tilde{x}(t) &= \sum_{k=-\infty}^{\infty}a_ke^{jk\omega_0 t},\quad \omega_0 =\frac{2\pi}{T}\\
                a_k &= \frac{1}{T}\int_{-T/2}^{T/2}\tilde{x}(t)e^{-jk\omega_0 t}dt.
            \end{align*}
            As $\tilde{x}(t) = x(t)$ for $|t| < T/2$, and also, as $x(t) = 0$ outside this interval,
            \begin{equation*}
                a_k = \frac{1}{T}\int_{-T/2}^{T/2}x(t)e^{-jk\omega_0 t}dt = \frac{1}{T}\int_{-\infty}^{\infty}x(t)e^{-jk\omega_0 t}dt.
            \end{equation*}
        \end{column}
        \begin{column}{0.5\textwidth}
            Defining the envelope $X(j\omega)$ of $Ta_k$ as        
            \begin{equation*}
                X(j\omega) = \int_{-\infty}^{\infty}x(t)e^{-j\omega t}dt,
            \end{equation*}
            we have, for the coefficients $a_k$, 
            \begin{equation*}
                a_k = \frac{1}{T}X(jk\omega_0).
            \end{equation*}
            Combining and expressing $\tilde{x}(t)$ in terms of $X(j\omega)$
            \begin{equation*}
                \tilde{x}(t) = \sum_{k=-\infty}^{\infty} \frac{1}{T}X(jk\omega_0)e^{jk\omega_0 t},
            \end{equation*}        
            or, as $\omega_0 =2\pi/T$    
            \begin{equation}
                \label{eq:xtildet_with_ft}
                \tilde{x}(t) = \frac{1}{2\pi}\sum_{k=-\infty}^{\infty} X(jk\omega_0)e^{jk\omega_0 t}\omega_0.
            \end{equation}             
        \end{column}        
    \end{columns}
\end{frame}


\begin{frame}
    \input{figures/fs_to_ft_integral}\par
    As $T\rightarrow \infty$, $\tilde{x}(t)$ approaches $x(t)$, and consequently, Eq.~\ref{eq:xtildet_with_ft} becomes a representation of $x(t)$. Furthermore, as $\omega_0 \rightarrow 0$ as $T \rightarrow \infty$, and the right-hand side of  Eq.~\ref{eq:xtildet_with_ft} passes to an integral. As $\omega_0 \rightarrow 0$, the summation converges to the integral of $X(j\omega)e^{j\omega t}$.
    
    \begin{tikzpicture}[remember picture,overlay]
        \node[draw=blue!50, fill=blue!10, inner sep=2pt,outer sep=2pt, rounded corners=0.1cm, anchor=north east, yshift=0cm, xshift=-1cm, text width=5cm]  at (current page.north east) {
            \begin{equation*}
                \tilde{x}(t) = \frac{1}{2\pi}\sum_{k=-\infty}^{\infty} X(jk\omega_0)e^{jk\omega_0 t}\omega_0.
            \end{equation*}
        Inverse Fourier transform:
        \begin{equation*}\label{eq:ift}
            x(t) = \frac{1}{2\pi}\int_{-\infty}^{\infty}X(j\omega)e^{j\omega t} d\omega.
        \end{equation*}
        Fourier transform or Fourier integral:
        \begin{equation*}\label{eq:ft}
            X(j\omega) = \int_{-\infty}^{\infty}x(t)e^{-j\omega t} dt.
        \end{equation*}
        } ;
    \end{tikzpicture}
\end{frame}