\section*{Equations}
\subsection*{Fourier}
{\centering
{\renewcommand{\arraystretch}{4}%
    \begin{tabular}{lcc}

    & CT & DT\\
        \cline{2-3}
    & Series (CT) & Series (DT)\\
    \cline{2-3}
    Periodic &
    $\begin{aligned}
        x(t) &= \sum_{k=-\infty}^{+\infty}a_k e^{jk\omega_0 t}\\
        a_k &= \frac{1}{T} \int_{T}x(t)e^{-jk\omega_0 t}dt
    \end{aligned}$\par

    &
    $\begin{aligned}
        x[n] &= \sum_{k=<N>}a_k e^{jk\left(\frac{2\pi}{N}\right) n}\\
        a_k &= \frac{1}{N} \sum_{n=<N>}x[n]e^{-jk\left(\frac{2\pi}{N}\right)n}
    \end{aligned}$\par
    \\[4ex]
        \cline{2-3}
     & Transform (CT) & Transform (DT)\\
    \cline{2-3}
    Aperiodic &
    $\begin{aligned}
        x(t) &= \frac{1}{2\pi}\int_{-\infty}^{+\infty} X(j\omega)e^{j\omega t}d\omega\\
        X(j\omega) &=  \int_{-\infty}^{+\infty}x(t)e^{-j\omega t}dt
    \end{aligned}$\par

    &


    $\begin{aligned}
        x[n] &= \frac{1}{2\pi}\int_{2\pi} X(e^{j\omega})e^{j\omega n}d\omega\\
        X(e^{j\omega}) &= \sum_{n=-\infty}^{+\infty}x[n]e^{-j\omega n}
    \end{aligned}$\par
    \\[4ex]
        \cline{2-3}
    \end{tabular}
    }
}
    \subsection*{Trigonometric Fourier Series}

    \begin{align*}
        x(t) &= a_0 + \sum_{k=1}^{\infty}a_k \cos(k\omega_0 t) + \sum_{k=1}^{\infty}b_k \sin(k\omega_0 t).\\
        a_0 &= \frac{1}{T}\int_T x(t)dt.\\
        a_k &= \frac{2}{T}\int_T x(t)\cos(k\omega_0 t)dt.\\
        b_k &= \frac{2}{T}\int_T x(t)\sin(k\omega_0 t)dt.
    \end{align*}
